@prefix qudt: <http://qudt.org/schema/qudt/> .
@prefix owl: <http://www.w3.org/2002/07/owl#> .
@prefix xsd: <http://www.w3.org/2001/XMLSchema#> .
@prefix fn: <http://www.w3.org/2005/xpath-functions#> .
@prefix skos: <http://www.w3.org/2004/02/skos/core#> .
@prefix nsp: <https://w3id.org/se/building/nsp#> .
@prefix rdfs: <http://www.w3.org/2000/01/rdf-schema#> .
@prefix path: <http://www.ontotext.com/path#> .
@prefix ref: <https://brickschema.org/schema/Brick/ref#> .
@prefix s223: <http://data.ashrae.org/standard223#> .
@prefix sh: <http://www.w3.org/ns/shacl#> .
@prefix dcterms: <http://purl.org/dc/terms/> .
@prefix bacnet: <http://data.ashrae.org/bacnet/2020#> .
@prefix brick: <https://brickschema.org/schema/Brick#> .
@prefix tag: <https://brickschema.org/schema/BrickTag#> .
@prefix rdf4j: <http://rdf4j.org/schema/rdf4j#> .
@prefix sosa: <http://www.w3.org/ns/sosa/> .
@prefix wgs: <http://www.w3.org/2003/01/geo/wgs84_pos#> .
@prefix bldg: <https://example.com/bldg#> .
@prefix gn: <http://www.geonames.org/ontology#> .
@prefix vcard: <http://www.w3.org/2006/vcard/ns#> .
@prefix unit: <http://qudt.org/vocab/unit/> .
@prefix rdf: <http://www.w3.org/1999/02/22-rdf-syntax-ns#> .
@prefix bsh: <https://brickschema.org/schema/BrickShape#> .
@prefix sesame: <http://www.openrdf.org/schema/sesame#> .
@prefix qudtqk: <http://qudt.org/vocab/quantitykind/> .
@prefix sdo: <http://schema.org/> .

skos:definition a owl:AnnotationProperty .

<https://w3id.org/se/building/nsp> a owl:Ontology;
  rdfs:label "NSP Ontology";
  owl:imports <https://brickschema.org/schema/Brick#> .

nsp:hasChild a owl:AsymmetricProperty, owl:IrreflexiveProperty, owl:ObjectProperty;
  skos:definition "A generic relation for child relationships." .

nsp:hasParent a owl:AsymmetricProperty, owl:IrreflexiveProperty, owl:ObjectProperty;
  skos:definition "A generic relation for parent relationships." .

nsp:hasAlarm a owl:AsymmetricProperty, owl:IrreflexiveProperty, owl:ObjectProperty;
  rdfs:subPropertyOf nsp:hasObject;
  rdfs:label "Has alarm";
  rdfs:seeAlso "The subject is associated with an EBO alarm identified by the object." .

nsp:hasObject a owl:AsymmetricProperty, owl:IrreflexiveProperty, owl:ObjectProperty;
  rdfs:label "Has object";
  skos:definition "The subject is associated with an EBO object identified by the object." .

nsp:hasPath a owl:AsymmetricProperty, owl:IrreflexiveProperty, owl:ObjectProperty,
    owl:FunctionalProperty;
  rdfs:label "Has path";
  skos:definition "The subject is either a representative of an EBO object or an EBO object property. The object is an identifier of an EBO path using a literal." .

nsp:hasProperty a owl:AsymmetricProperty, owl:IrreflexiveProperty, owl:ObjectProperty,
    owl:FunctionalProperty;
  rdfs:label "Has property";
  skos:definition "The subject is associated with an EBO property identified by the object." .

nsp:hasPropertyOnObject a owl:AsymmetricProperty, owl:IrreflexiveProperty, owl:ObjectProperty,
    owl:FunctionalProperty;
  rdfs:subPropertyOf nsp:hasObject;
  rdfs:label "Has property on object";
  skos:definition """The subject is associated with an EBO property on an object identified by the object.

I.e the property part is not part of the semantic object identifier.""" .

nsp:hasServer a owl:AsymmetricProperty, owl:IrreflexiveProperty, owl:ObjectProperty,
    owl:FunctionalProperty;
  rdfs:label "Has server";
  skos:definition """The subject is associated with an EBO server identified by the object.

I.e the property part is not part of the semantic object identifier.""" .

nsp:hasSchedule a owl:AsymmetricProperty, owl:IrreflexiveProperty, owl:ObjectProperty;
  rdfs:subPropertyOf nsp:hasObject;
  rdfs:label "Has schedule";
  skos:definition "The subject is associated with an EBO schedule identified by the object." .

nsp:hasTrendLog a owl:AsymmetricProperty, owl:IrreflexiveProperty, owl:ObjectProperty;
  rdfs:subPropertyOf nsp:hasObject;
  rdfs:label "Has trendlog";
  skos:definition "The subject is associated with an EBO trend log identified by the object." .

nsp:hasPresentation a owl:AsymmetricProperty, owl:IrreflexiveProperty, owl:ObjectProperty;
  rdfs:subPropertyOf nsp:hasObject;
  rdfs:label "Has presenatation";
  skos:definition "The subject is associated with an EBO presentation identified by the object." .

nsp:removeProperty a owl:AsymmetricProperty, owl:IrreflexiveProperty, owl:ObjectProperty;
  rdfs:label "Remove property";
  skos:definition "Removes an inherited property." .

nsp:Entity a owl:Class .

nsp:EntityProperty a owl:Class;
  rdfs:subClassOf owl:ObjectProperty .

brick:hasPart rdfs:subPropertyOf nsp:hasChild .

brick:feeds rdfs:subPropertyOf nsp:hasChild .

brick:meters rdfs:subPropertyOf nsp:hasParent .

brick:isMeteredBy rdfs:subPropertyOf nsp:hasChild .

brick:hasLocation rdfs:subPropertyOf nsp:hasParent .

brick:hasSubMeter rdfs:subPropertyOf nsp:hasChild .

brick:isSubMeterOf rdfs:subPropertyOf nsp:hasParent .

brick:isLocationOf rdfs:subPropertyOf nsp:hasChild .

brick:isFedBy rdfs:subPropertyOf nsp:hasParent .

brick:isPointOf rdfs:subPropertyOf nsp:hasParent .

brick:hasPoint rdfs:subPropertyOf nsp:hasChild .

brick:isPartOf rdfs:subPropertyOf nsp:hasParent .

brick:isRegulatedBy rdfs:subPropertyOf nsp:hasParent .

brick:Equipment rdfs:subClassOf nsp:Entity .

brick:Location rdfs:subClassOf nsp:Entity .

brick:Collection rdfs:subClassOf nsp:Entity .

brick:EntityProperty rdfs:subClassOf nsp:EntityProperty .

brick:Point rdfs:subClassOf nsp:Entity .

brick:hasAddress rdfs:subClassOf nsp:EntityProperty .

brick:hasUnit rdfs:subClassOf nsp:EntityProperty .

brick:Measurable rdfs:subClassOf nsp:Entity .

brick:Meter nsp:removeProperty brick:isMeteredBy .
